src/main.fst
@@ -13,23 +13,102 @@ module ST = FStar.HyperStack.ST
 module U32 = FStar.UInt32
 module U8 = FStar.UInt8
 
+// https://docs.oasis-open.org/mqtt/mqtt/v5.0/os/mqtt-v5.0-os.html#_Toc3901022
+// 2.1.2 MQTT Control Packet type
+// Table 2‑1 MQTT Control Packet types
+type type_mqtt_control_packets = U8.t // Base 10
+
+let define_mqtt_control_packet_RESERVED : type_mqtt_control_packets = 0uy
+let define_mqtt_control_packet_CONNECT : type_mqtt_control_packets = 1uy
+let define_mqtt_control_packet_CONNACK : type_mqtt_control_packets = 2uy
+let define_mqtt_control_packet_PUBLISH : type_mqtt_control_packets = 3uy
+let define_mqtt_control_packet_PUBACK : type_mqtt_control_packets = 4uy
+let define_mqtt_control_packet_PUBREC : type_mqtt_control_packets = 5uy
+let define_mqtt_control_packet_PUBREL : type_mqtt_control_packets = 6uy
+let define_mqtt_control_packet_PUBCOMP : type_mqtt_control_packets = 7uy
+let define_mqtt_control_packet_SUBSCRIBE : type_mqtt_control_packets = 8uy
+let define_mqtt_control_packet_SUBACK : type_mqtt_control_packets = 9uy
+let define_mqtt_control_packet_UNSUBSCRIBE : type_mqtt_control_packets = 10uy
+let define_mqtt_control_packet_UNSUBACK : type_mqtt_control_packets = 11uy
+let define_mqtt_control_packet_PINGREQ : type_mqtt_control_packets = 12uy
+let define_mqtt_control_packet_PINGRESP : type_mqtt_control_packets = 13uy
+let define_mqtt_control_packet_DISCONNECT : type_mqtt_control_packets = 14uy
+let define_mqtt_control_packet_AUTH : type_mqtt_control_packets = 15uy
+
+// https://docs.oasis-open.org/mqtt/mqtt/v5.0/os/mqtt-v5.0-os.html#_Toc3901022
+// 2.1.3 Flags
+// Table 2‑2 Flag Bits
+type type_flags = U8.t // Base 2
+
+let define_flag_CONNECT : type_flags = 0b0000uy
+let define_flag_CONNACK : type_flags = 0b0000uy 
+// PUBLISH は下記に記述
+let define_flag_PUBACK : type_flags = 0b0000uy
+let define_flag_PUBREC : type_flags = 0b0000uy
+let define_flag_PUBREL : type_flags = 0b0010uy
+let define_flag_PUBCOMP : type_flags = 0b0000uy
+let define_flag_SUBSCRIBE : type_flags = 0b0010uy
+let define_flag_SUBACK : type_flags = 0b0000uy
+let define_flag_UNSUBSCRIBE : type_flags = 0b0010uy
+let define_flag_UNSUBACK : type_flags = 0b0000uy
+let define_flag_PINGREQ : type_flags = 0b0000uy
+let define_flag_PINGRESP : type_flags = 0b0000uy
+let define_flag_DISCONNECT : type_flags = 0b0000uy
+let define_flag_AUTH : type_flags = 0b0000uy
+
+// https://docs.oasis-open.org/mqtt/mqtt/v5.0/os/mqtt-v5.0-os.html
+// 3.3.1.1 DUP
+type type_dup_flags = U8.t // Base 10
+
+let define_dup_flag_first_delivery : type_dup_flags = 0uy
+let define_dup_flag_re_delivery : type_dup_flags = 1uy 
+
+// https://docs.oasis-open.org/mqtt/mqtt/v5.0/os/mqtt-v5.0-os.html
+// 3.3.1.2 QoS
+// Table 3‑2 - QoS definitions
+type type_qos_flags = U8.t // Base 2
+
+let define_qos_flag_at_most_once_delivery : type_qos_flags = 0b00uy
+let define_qos_flag_at_least_once_delivery : type_qos_flags = 0b01uy
+let define_qos_flag_exactly_once_delivery : type_qos_flags = 0b10uy
+let define_qos_flag_reserved : type_qos_flags = 0b11uy
+
+// https://docs.oasis-open.org/mqtt/mqtt/v5.0/os/mqtt-v5.0-os.html
+// 3.3.1.3 RETAIN
+type type_retain_flags = U8.t // Base 10
+
+let define_retain_flag_must_not_store_application_message : type_retain_flags = 0uy
+let define_retain_flag_must_store_application_message : type_retain_flags = 1uy 
+
+
 // debug tool
-assume val print_hex (i: U8.t{ 0 <= U8.v i /\ U8.v i <= 255}): Stack unit
+assume val extern_print_hex (i: U8.t{ 0 <= U8.v i /\ U8.v i <= 255}): Stack unit
   (requires (fun h -> true))
   (ensures (fun h0 ret h1 -> true))
-// ---
 
-val normal_loop: src:B.buffer U8.t -> len:U32.t -> Stack C.exit_code
+// ex. 0xab -> 0x0a TODO: rの定義域を追加
+val get_most_significant_four_bit: i:U8.t -> r:U8.t
+let get_most_significant_four_bit i = U8.shift_right i 4ul
+
+// ex. 0xab -> 0x0b TODO: rの定義域を追加
+val get_least_significant_four_bit: i:U8.t -> r:U8.t
+let get_least_significant_four_bit i = U8.logand i 0x0fuy
+
+val bytes_loop: src:B.buffer U8.t -> len:U32.t -> Stack C.exit_code
   (requires fun h0 -> B.live h0 src /\ B.length src = U32.v len )
   (ensures fun _ _ _ -> true)
-let normal_loop src len =
+let bytes_loop src len =
   let inv h (i: nat) = B.live h src in
   let body (i: U32.t{ 0 <= U32.v i /\ U32.v i < U32.v len }): Stack unit
     (requires (fun h -> inv h (U32.v i)))
     (ensures (fun _ _ _ -> true))
   =
-    let v : U8.t = src.(i) in
-      print_hex v
+    let oneByte : U8.t = src.(i) in
+      let most_significant_four_bit = get_most_significant_four_bit in 
+      let least_significant_four_bit = get_least_significant_four_bit in 
+      extern_print_hex (oneByte);
+      extern_print_hex (get_most_significant_four_bit oneByte);
+      extern_print_hex (get_least_significant_four_bit oneByte)
   in
   C.Loops.for 0ul len inv body;
   (* return *) C.EXIT_SUCCESS
@@ -44,6 +123,6 @@ val parse (request: B.buffer U8.t) (len: U32.t):
 
 let parse request len =
     push_frame ();
-    let r = normal_loop request len in
+    let r = bytes_loop request len in
     pop_frame ();
     C.EXIT_SUCCESS
